<?xml version="1.0"?>
<rdf:RDF xmlns="http://slipo.eu/def/fusion/#"
     xml:base="http://slipo.eu/def/fusion/"
     xmlns:rdf="http://www.w3.org/1999/02/22-rdf-syntax-ns#"
     xmlns:terms="http://purl.org/dc/terms/"
     xmlns:owl="http://www.w3.org/2002/07/owl#"
     xmlns:xml="http://www.w3.org/XML/1998/namespace"
     xmlns:slipo="http://slipo.eu/def#"
     xmlns:xsd="http://www.w3.org/2001/XMLSchema#"
     xmlns:skos="http://www.w3.org/2004/02/skos/core#"
	 xmlns:prov="http://www.w3.org/ns/prov#"
     xmlns:rdfs="http://www.w3.org/2000/01/rdf-schema#"
     xmlns:dc="http://purl.org/dc/elements/1.1/">
    <owl:Ontology rdf:about="">
        <owl:imports rdf:resource="https://raw.githubusercontent.com/SLIPO-EU/poi-data-model/master/poi-model.owl"/>
        <rdfs:comment>Extension of SLIPO data model for representing fused POIs and their provenance.</rdfs:comment>
        <owl:versionInfo xml:lang="en">1.0.0</owl:versionInfo>
    </owl:Ontology>
	
	
    <!-- 
    ///////////////////////////////////////////////////////////////////////////////////////
    //
    // Classes
    //
    ///////////////////////////////////////////////////////////////////////////////////////
     -->
	 
    <!-- http://slipo.eu/def#fusedPOI -->

    <owl:Class rdf:about="http://slipo.eu/def#fusedPOI">
        <rdfs:label>fusedPOI</rdfs:label>
        <rdfs:subClassOf rdf:resource="http://slipo.eu/def#POI"/>
		<rdfs:subClassOf>
            <owl:Restriction>
                <owl:onProperty rdf:resource="http://slipo.eu/def#fusion-confidence"/>
                <owl:qualifiedCardinality rdf:datatype="http://www.w3.org/2001/XMLSchema#nonNegativeInteger">1</owl:qualifiedCardinality>
                <owl:onDataRange rdf:resource="http://www.w3.org/2001/XMLSchema#float"/>
            </owl:Restriction>
        </rdfs:subClassOf>
		<rdfs:subClassOf>
            <owl:Restriction>
                <owl:onProperty rdf:resource="http://slipo.eu/def#fusion-gain"/>
                <owl:qualifiedCardinality rdf:datatype="http://www.w3.org/2001/XMLSchema#nonNegativeInteger">1</owl:qualifiedCardinality>
                <owl:onDataRange rdf:resource="http://www.w3.org/2001/XMLSchema#float"/>
            </owl:Restriction>
        </rdfs:subClassOf>
        <rdfs:comment xml:lang="en">The class of a POI from two input resources and the actions applied to generate its properties.</rdfs:comment>
    </owl:Class>
	
	
	<!-- http://www.w3.org/ns/prov#appliedAgent -->

    <owl:Class rdf:about="http://www.w3.org/ns/prov#appliedAgent">
        <rdfs:label>appliedAgent</rdfs:label>
        <rdfs:subClassOf rdf:resource="http://www.w3.org/ns/prov#Agent"/>
		<rdfs:subClassOf>
            <owl:Restriction>
                <owl:onProperty rdf:resource="http://www.w3.org/ns/prov#attribute"/>
                <owl:maxQualifiedCardinality rdf:datatype="http://www.w3.org/2001/XMLSchema#nonNegativeInteger">2</owl:maxQualifiedCardinality>
                <owl:onDataRange rdf:resource="http://www.w3.org/2001/XMLSchema#string"/>
            </owl:Restriction>
        </rdfs:subClassOf>
		<rdfs:subClassOf>
            <owl:Restriction>
                <owl:onProperty rdf:resource="http://www.w3.org/ns/prov#fusion-action"/>
                <owl:qualifiedCardinality rdf:datatype="http://www.w3.org/2001/XMLSchema#nonNegativeInteger">1</owl:qualifiedCardinality>
                <owl:onDataRange rdf:resource="http://www.w3.org/2001/XMLSchema#string"/>
            </owl:Restriction>
        </rdfs:subClassOf>
		<rdfs:subClassOf>
            <owl:Restriction>
                <owl:onProperty rdf:resource="http://www.w3.org/ns/prov#left-value"/>
                <owl:qualifiedCardinality rdf:datatype="http://www.w3.org/2001/XMLSchema#nonNegativeInteger">1</owl:qualifiedCardinality>
                <owl:onDataRange rdf:resource="http://www.w3.org/2001/XMLSchema#string"/>
            </owl:Restriction>
        </rdfs:subClassOf>
		<rdfs:subClassOf>
            <owl:Restriction>
                <owl:onProperty rdf:resource="http://www.w3.org/ns/prov#right-value"/>
                <owl:qualifiedCardinality rdf:datatype="http://www.w3.org/2001/XMLSchema#nonNegativeInteger">1</owl:qualifiedCardinality>
                <owl:onDataRange rdf:resource="http://www.w3.org/2001/XMLSchema#string"/>
            </owl:Restriction>
        </rdfs:subClassOf>
		<rdfs:subClassOf>
            <owl:Restriction>
                <owl:onProperty rdf:resource="http://www.w3.org/ns/prov#fused-value"/>
                <owl:qualifiedCardinality rdf:datatype="http://www.w3.org/2001/XMLSchema#nonNegativeInteger">1</owl:qualifiedCardinality>
                <owl:onDataRange rdf:resource="http://www.w3.org/2001/XMLSchema#string"/>
            </owl:Restriction>
        </rdfs:subClassOf>
        <rdfs:comment xml:lang="en">The class of an Agent representing provenance of a particular property (POI attribute) after a fusion action is applied.</rdfs:comment>
    </owl:Class>

	<!-- http://www.w3.org/ns/prov#derivedAgent -->

    <owl:Class rdf:about="http://www.w3.org/ns/prov#derivedAgent">
        <rdfs:label>derivedAgent</rdfs:label>
        <rdfs:subClassOf rdf:resource="http://www.w3.org/ns/prov#Agent"/>
		<rdfs:subClassOf>
            <owl:Restriction>
                <owl:onProperty rdf:resource="http://www.w3.org/ns/prov#right-uri"/>
                <owl:qualifiedCardinality rdf:datatype="http://www.w3.org/2001/XMLSchema#nonNegativeInteger">1</owl:qualifiedCardinality>
                <owl:onDataRange rdf:resource="http://www.w3.org/2001/XMLSchema#string"/>
            </owl:Restriction>
        </rdfs:subClassOf>
		<rdfs:subClassOf>
            <owl:Restriction>
                <owl:onProperty rdf:resource="http://www.w3.org/ns/prov#default-fusion-action"/>
                <owl:qualifiedCardinality rdf:datatype="http://www.w3.org/2001/XMLSchema#nonNegativeInteger">1</owl:qualifiedCardinality>
                <owl:onDataRange rdf:resource="http://www.w3.org/2001/XMLSchema#string"/>
            </owl:Restriction>
        </rdfs:subClassOf>
		<rdfs:subClassOf>
            <owl:Restriction>
                <owl:onProperty rdf:resource="http://www.w3.org/ns/prov#validation-action"/>
                <owl:qualifiedCardinality rdf:datatype="http://www.w3.org/2001/XMLSchema#nonNegativeInteger">1</owl:qualifiedCardinality>
                <owl:onDataRange rdf:resource="http://www.w3.org/2001/XMLSchema#string"/>
            </owl:Restriction>
        </rdfs:subClassOf>		
		<rdfs:subClassOf>
            <owl:Restriction>
                <owl:onProperty rdf:resource="http://www.w3.org/ns/prov#fusion-confidence"/>
                <owl:qualifiedCardinality rdf:datatype="http://www.w3.org/2001/XMLSchema#nonNegativeInteger">1</owl:qualifiedCardinality>
                <owl:onDataRange rdf:resource="http://www.w3.org/2001/XMLSchema#string"/>
            </owl:Restriction>
        </rdfs:subClassOf>
        <rdfs:comment xml:lang="en">The class of an Agent representing provenance of a fused POI.</rdfs:comment>
    </owl:Class>
	
	
    <!-- 
    ///////////////////////////////////////////////////////////////////////////////////////
    //
    // Object Properties
    //
    ///////////////////////////////////////////////////////////////////////////////////////
     -->
	
    <!-- http://www.w3.org/ns/prov#appliedAction -->

    <owl:ObjectProperty rdf:about="http://www.w3.org/ns/prov#appliedAction">
        <rdfs:domain rdf:resource="http://slipo.eu/def#fusedPOI"/>
        <rdfs:range rdf:resource="http://www.w3.org/ns/prov#appliedAgent"/>
        <rdfs:comment xml:lang="en">Keeps track of the fusion action applied on values from two input POI resources regarding a specific attribute (e.g., fusing phone numbers).</rdfs:comment>
    </owl:ObjectProperty>


	<!-- http://www.w3.org/ns/prov#wasDerivedFrom -->

    <owl:ObjectProperty rdf:about="http://www.w3.org/ns/prov#wasDerivedFrom">
        <rdfs:domain rdf:resource="http://slipo.eu/def#fusedPOI"/>
        <rdfs:range rdf:resource="http://www.w3.org/ns/prov#derivedAgent"/>
        <rdfs:comment xml:lang="en">Keeps track of the fusion applied on two input POI resources.</rdfs:comment>
    </owl:ObjectProperty>
	

    <!-- 
    ///////////////////////////////////////////////////////////////////////////////////////
    //
    // Data properties
    //
    ///////////////////////////////////////////////////////////////////////////////////////
     -->

	<!-- http://www.w3.org/ns/prov#attribute -->

    <owl:DatatypeProperty rdf:about="http://www.w3.org/ns/prov#attribute">
        <rdfs:domain rdf:resource="http://www.w3.org/ns/prov#appliedAgent"/>
        <rdfs:range rdf:resource="http://www.w3.org/2001/XMLSchema#string"/>
        <rdfs:comment xml:lang="en">The property (attribute name) involved in the fusion action.</rdfs:comment>
    </owl:DatatypeProperty>

	<!-- http://www.w3.org/ns/prov#fusion-action -->

    <owl:DatatypeProperty rdf:about="http://www.w3.org/ns/prov#fusion-action">
        <rdfs:domain rdf:resource="http://www.w3.org/ns/prov#appliedAgent"/>
        <rdfs:range rdf:resource="http://www.w3.org/2001/XMLSchema#string"/>
        <rdfs:comment xml:lang="en">The fusion action to be applied on the two input property values.</rdfs:comment>
    </owl:DatatypeProperty>
	
	<!-- http://www.w3.org/ns/prov#left-value -->

    <owl:DatatypeProperty rdf:about="http://www.w3.org/ns/prov#left-value">
        <rdfs:domain rdf:resource="http://www.w3.org/ns/prov#appliedAgent"/>
        <rdfs:range rdf:resource="http://www.w3.org/2001/XMLSchema#string"/>
        <rdfs:comment xml:lang="en">The value of the first POI (left part in the fusion action) on the examined property (attribute).</rdfs:comment>
    </owl:DatatypeProperty>

	<!-- http://www.w3.org/ns/prov#right-value -->

    <owl:DatatypeProperty rdf:about="http://www.w3.org/ns/prov#right-value">
        <rdfs:domain rdf:resource="http://www.w3.org/ns/prov#appliedAgent"/>
        <rdfs:range rdf:resource="http://www.w3.org/2001/XMLSchema#string"/>
        <rdfs:comment xml:lang="en">The value of the second POI (right part in the fusion action) on the examined property (attribute).</rdfs:comment>
    </owl:DatatypeProperty>

	<!-- http://www.w3.org/ns/prov#fused-value -->

    <owl:DatatypeProperty rdf:about="http://www.w3.org/ns/prov#fused-value">
        <rdfs:domain rdf:resource="http://www.w3.org/ns/prov#appliedAgent"/>
        <rdfs:range rdf:resource="http://www.w3.org/2001/XMLSchema#string"/>
        <rdfs:comment xml:lang="en">The resulting value of the POI on the examined property (attribute) after fusion.</rdfs:comment>
    </owl:DatatypeProperty>
	
	<!-- http://www.w3.org/ns/prov#left-uri -->

    <owl:DatatypeProperty rdf:about="http://www.w3.org/ns/prov#left-uri">
        <rdfs:domain rdf:resource="http://www.w3.org/ns/prov#derivedAgent"/>
        <rdfs:range rdf:resource="http://www.w3.org/2001/XMLSchema#string"/>
        <rdfs:comment xml:lang="en">The URI of the first POI (left part) involved in the fusion.</rdfs:comment>
    </owl:DatatypeProperty>

	<!-- http://www.w3.org/ns/prov#right-uri -->

    <owl:DatatypeProperty rdf:about="http://www.w3.org/ns/prov#right-uri">
        <rdfs:domain rdf:resource="http://www.w3.org/ns/prov#derivedAgent"/>
        <rdfs:range rdf:resource="http://www.w3.org/2001/XMLSchema#string"/>
        <rdfs:comment xml:lang="en">The URI of the second POI (right part) involved in the fusion.</rdfs:comment>
    </owl:DatatypeProperty>

	<!-- http://www.w3.org/ns/prov#default-fusion-action -->

    <owl:DatatypeProperty rdf:about="http://www.w3.org/ns/prov#default-fusion-action">
        <rdfs:domain rdf:resource="http://www.w3.org/ns/prov#derivedAgent"/>
        <rdfs:range rdf:resource="http://www.w3.org/2001/XMLSchema#string"/>
        <rdfs:comment xml:lang="en">The default fusion action (keep-left, keep-both, etc.) to be applied on the two input property values if no other specific action or condition is defined.</rdfs:comment>
    </owl:DatatypeProperty>
	
	<!-- http://www.w3.org/ns/prov#validation-action -->

    <owl:DatatypeProperty rdf:about="http://www.w3.org/ns/prov#validation-action">
        <rdfs:domain rdf:resource="http://www.w3.org/ns/prov#derivedAgent"/>
        <rdfs:range rdf:resource="http://www.w3.org/2001/XMLSchema#string"/>
        <rdfs:comment xml:lang="en">The result of the validation rule (accept, reject, accept-mark-ambiguous, etc.) applied on the link between two input POI resources.</rdfs:comment>
    </owl:DatatypeProperty>

    <!-- http://www.w3.org/ns/prov#fusion-confidence -->

    <owl:DatatypeProperty rdf:about="http://www.w3.org/ns/prov#fusion-confidence">
        <rdfs:domain rdf:resource="http://www.w3.org/ns/prov#derivedAgent"/>
        <rdfs:range rdf:resource="http://www.w3.org/2001/XMLSchema#string"/>
        <rdfs:comment xml:lang="en">The confidence measure of the applied fusion over the two input POI resources.</rdfs:comment>
    </owl:DatatypeProperty>
	
	
    <!-- http://slipo.eu/def#fusion-gain -->

    <owl:DatatypeProperty rdf:about="http://slipo.eu/def#fusion-gain">
        <rdfs:domain rdf:resource="http://slipo.eu/def#fusedPOI"/>
        <rdfs:range rdf:resource="http://www.w3.org/2001/XMLSchema#float"/>
        <rdfs:comment xml:lang="en">Fusion attribute gain.</rdfs:comment>
    </owl:DatatypeProperty>
    
    <!-- http://slipo.eu/def#fusion-confidence -->

    <owl:DatatypeProperty rdf:about="http://slipo.eu/def#fusion-confidence">
        <rdfs:domain rdf:resource="http://slipo.eu/def#fusedPOI"/>
        <rdfs:range rdf:resource="http://www.w3.org/2001/XMLSchema#float"/>
        <rdfs:comment xml:lang="en">Fusion confidence.</rdfs:comment>
    </owl:DatatypeProperty>

</rdf:RDF>
